Matroid/ForMathlib/Set.lean
@@ -54,3 +54,59 @@ theorem diff_eq_diff_inter_of_subset {s t : Set α} (h : s ⊆ t) (r : Set α) :
 theorem diff_union_eq_union_of_subset (s : Set α) {t r : Set α} (h : t ⊆ r) :
     (s \ t) ∪ r = s ∪ r := by
   ext x; simp only [mem_union, mem_diff]; tauto
+
+
+theorem diff_eq_diff_iff_inter_eq_inter {s t r : Set α} : s \ t = s \ r ↔ (t ∩ s = r ∩ s) := by
+  rw [← diff_inter_self_eq_diff, ← diff_inter_self_eq_diff (t := r)]
+  refine' ⟨fun h ↦ _, fun h ↦ by rw [h]⟩
+  rw [← diff_diff_cancel_left (inter_subset_right t s), h,
+    diff_diff_cancel_left (inter_subset_right r s)]
+
+@[simp] theorem diff_inter_diff_right {s t r : Set α} : (t \ s) ∩ (r \ s) = (t ∩ r) \ s := by
+  simp only [diff_eq, inter_assoc, inter_comm sᶜ, inter_self]
+
+theorem inter_diff_right_comm {s t r : Set α} : (s ∩ t) \ r = (s \ r) ∩ t := by
+  simp_rw [diff_eq, inter_right_comm]
+
+theorem pair_diff_left {x y : α} (hne : x ≠ y) : ({x, y} : Set α) \ {x} = {y} := by
+  rw [insert_diff_of_mem _ (by exact rfl : x ∈ {x}), diff_singleton_eq_self (by simpa)]
+
+theorem pair_diff_right {x y : α} (hne : x ≠ y) : ({x, y} : Set α) \ {y} = {x} := by
+  rw [pair_comm, pair_diff_left hne.symm]
+
+@[simp] theorem pair_subset_iff {x y : α} {s : Set α} : {x,y} ⊆ s ↔ x ∈ s ∧ y ∈ s := by
+  rw [insert_subset_iff, singleton_subset_iff]
+
+theorem pair_subset {x y : α} {s : Set α} (hx : x ∈ s) (hy : y ∈ s) : {x,y} ⊆ s :=
+  pair_subset_iff.2 ⟨hx,hy⟩
+
+theorem subset_insert_iff {s t : Set α} {x : α} :
+    s ⊆ insert x t ↔ s ⊆ t ∨ (x ∈ s ∧ s \ {x} ⊆ t) := by
+  rw [← diff_singleton_subset_iff]
+  obtain (hx | hx) := em (x ∈ s)
+  · rw [and_iff_right hx]
+    exact ⟨fun h ↦ Or.inr h, fun h ↦ h.elim (fun hst ↦ (diff_subset _ _).trans hst) id⟩
+  rw [diff_singleton_eq_self hx]
+  tauto
+
+theorem Nonempty.subset_pair_iff {x y : α} {s : Set α} (hs : s.Nonempty) :
+    s ⊆ {x,y} ↔ s = {x} ∨ s = {y} ∨ s = {x,y} := by
+  obtain (rfl | hne) := eq_or_ne x y
+  · rw [pair_eq_singleton, hs.subset_singleton_iff]; simp
+  rw [subset_insert_iff, subset_singleton_iff_eq, subset_singleton_iff_eq, diff_eq_empty,
+    iff_false_intro hs.ne_empty, false_or, and_or_left, ← singleton_subset_iff,
+    ← subset_antisymm_iff, eq_comm (b := s), ← or_assoc, or_comm (a := s = _), or_assoc]
+  convert Iff.rfl using 3
+  rw [Iff.comm, subset_antisymm_iff, diff_subset_iff, subset_diff, disjoint_singleton,
+    and_iff_left hne.symm, ← and_assoc, and_comm, singleton_union, ← and_assoc, ← union_subset_iff,
+    singleton_union, pair_comm, ← subset_antisymm_iff, eq_comm]
+
+theorem inter_insert_eq {A : Set α} {b c : α} (hne : b ≠ c):
+    (insert b A) ∩ (insert c A) = A := by
+  rw [insert_eq, insert_eq, ← inter_union_distrib_right, Disjoint.inter_eq _, empty_union]
+  rwa [disjoint_singleton]
+
+theorem union_insert_eq {A : Set α} {b c : α} :
+    (insert b A) ∪ (insert c A) = insert c (insert b A) := by
+  rw [insert_eq, insert_eq, ← union_union_distrib_right, @union_comm _ {b} _,
+    union_assoc, ← insert_eq, ← insert_eq]
